Total/Stlc/Lang/Surface/Grammar.lean
@@ -4,7 +4,6 @@ namespace Total.Stlc.Lang.Surface
   inductive Ty: Type where
     | bool: Ty
     | nat: Ty
-    -- | fn (dom: List Ty) (rng: Ty): Ty
 
   inductive UnOp: Type where
     | not: UnOp
@@ -27,14 +26,6 @@ namespace Total.Stlc.Lang.Surface
     | unOp (op: UnOp) (operand: Term): Term
     | binOp (op: BinOp) (lhs rhs: Term): Term
     | cond (c t f: Term): Term
-    -- | var  (id: String): Term
-    -- | bind (id: String) (ty: Ty) (expr: Term) (scope: Term): Term
-    -- | abs (params: List (String × Ty)) (body: Term): Term
-    -- | app (fn: Term) (args: List Term): Term
 
   inductive Top: Type where
-    -- | val (id: String) (ty: Ty) (value: Term): Top
-    -- | defn (id: String) (args: List (String × Ty)) (body: Term): Top
-    -- | letVal (id: String) (ty: Ty) (value: Term): Top
-    -- | letDefn (id: String) (args: List (String × Ty)) (body: Term): Top
 namespace Total.Stlc.Lang.Surface
